src/named/SimpleEvalCtx.v
@@ -11,9 +11,7 @@ Import Core.Notations.
 
 Require Coq.derive.Derive.
 
-Set Default Proof Mode "Classic".
 
-(*An extension to subst_lang *)
 Definition subst_eval_ctx :=
   [(* TODO: do I want a substitution eval ctx? I think no
          [:> "G1" : #"env", "G2" : #"env", "G3" : #"env", "f" : #"sub" %"G1" %"G2", "g" : #"sub" %"G2" %"G3", "A" : #"ty", "e" : #"el" %"G3" %"A"
@@ -50,122 +48,13 @@ Definition subst_eval_ctx :=
      ]
   ]%arule.
 
-(*TODO: move to utils*)
-Lemma nth_tail_length_app A (l1 l2 : list A) n
-  : n = length l1 ->
-    nth_tail n (l1++l2) = l2.
-Proof.
-  intros; subst.
-  induction l1; basic_goal_prep; basic_utils_crush.
-Qed.
-
-Lemma nth_tail_app A n (l l' : list A)
-  : n < length l ->
-    nth_tail n (l++l') = (nth_tail n l)++l'.
-Admitted.
-
-Lemma nth_tail_is_cons_bounds_n A n (l l' : list A) p
-  : nth_tail n l = p::l' ->
-    n < length l.
-Admitted.
-
-(*TODO: move to elab*)
-Lemma elab_lang_cons_nth_tail_app
-     : forall (n : nat) (l el l' el' el'' : list (string * rule)) (name : string) (r er : rule),
-       nth_error l n = Some (name, r) ->
-       nth_tail n el = (name, er) :: el'' ->
-       fresh name (nth_tail (S n) (l++l')) ->
-       elab_lang (nth_tail (S n) (l++l')) (nth_tail (S n) (el++el')) ->
-       elab_rule (nth_tail (S n) (el++el')) r er ->
-       elab_lang (nth_tail n (l++l')) (nth_tail n (el++el')).
-Proof.
-  intros.
-  eapply elab_lang_cons_nth_tail; eauto.
-  {
-    rewrite nth_error_app1; eauto.
-    apply nth_error_Some.
-    intro H'.
-    rewrite H in H'.
-    inversion H'.
-  }
-  {
-    rewrite nth_tail_app.
-    rewrite H0.
-    reflexivity.
-    eapply nth_tail_is_cons_bounds_n; eauto.
-  }
-Qed.
-    
-
-(*TODO: move back to elab*)
-Ltac break_down_elab_lang' :=
-  repeat ((eapply elab_lang_cons_nth_tail_app
-           || eapply elab_lang_cons_nth_tail);
-              [compute; reflexivity
-              | compute; reflexivity
-              | apply use_compute_fresh; compute; reflexivity
-              | ..]);
-  [solve [assumption | compute; apply elab_lang_nil]|..].
-
-Local Ltac t :=
-  match goal with
-  | [|- fresh _ _ ]=> apply use_compute_fresh; compute; reflexivity
-  | [|- sublist _ _ ]=> apply (use_compute_sublist string_dec); compute; reflexivity
-  | [|- In _ _ ]=> apply named_list_lookup_err_in; compute; reflexivity
-  | [|- len_eq _ _] => econstructor
-  | [|-elab_sort _ _ _ _] => eapply elab_sort_by
-  | [|-elab_ctx _ _ _] => econstructor
-  | [|-elab_args _ _ _ _ _ _] => eapply elab_args_cons_ex' || econstructor
-  | [|-elab_term _ _ _ _ _] => eapply elab_term_var || eapply elab_term_by'
-  | [|-wf_term _ _ _ _] => shelve
-  | [|-elab_rule _ _ _] => econstructor
-  | [|- _ = _] => compute; reflexivity
-  end.
+Derive eval_ctx_elab
+       SuchThat (Pre.elab_lang subst_elab subst_eval_ctx eval_ctx_elab)
+       As eval_ctx_wf.
+Proof. auto_elab. Qed.
+#[export] Hint Resolve eval_ctx_wf : elab_pfs.
 
 
-Ltac auto_elab' :=
-  match goal with
-  | [|- elab_lang ?l ?el] =>
-  rewrite (as_nth_tail l);
-  rewrite (as_nth_tail el);
-  break_down_elab_lang';
-  unshelve solve[repeat t];
-  cleanup_auto_elab
-  end.
-
-Derive subst_eval_ctx_elab
-       SuchThat (elab_lang (subst_eval_ctx++subst_lang) (subst_eval_ctx_elab ++ subst_elab))
-       As subst_eval_ctx_wf.
-Proof.
-  pose proof subst_lang_wf.
-  match goal with
-  | [|- elab_lang ?l ?el] =>
-  rewrite (as_nth_tail l);
-    rewrite (as_nth_tail el)
-  end.
-  repeat ((eapply elab_lang_cons_nth_tail_app
-           || eapply elab_lang_cons_nth_tail);
-              [compute; reflexivity
-              | compute; reflexivity
-              | apply use_compute_fresh; compute; reflexivity
-              | ..]).
-  
-  rewrite !nth_tail_length_app; [assumption|..].
-  cbn.
-  match goal with
-    [ |-context [length ?emp]] => unify emp (@nil (string*rule))
-  end.
-  reflexivity.
-  reflexivity.
-  
-  all:unshelve solve[repeat t];
-  cleanup_auto_elab.
-  
-Qed.
-
-Axiom TODO : False.
-
-(*an extension to subst_eval_ctx++stlc*)
 Definition Estlc :=  
   [
      [:> "G" : #"env",
@@ -211,35 +100,9 @@ Definition Estlc :=
        #"Eapp_l" "E" "e'" : #"Ectx" %"G" %"C" %"B"
   ]]%arule.
 
-
 Derive Estlc_elab
-       SuchThat (elab_lang (Estlc++subst_eval_ctx++stlc)
-                           (Estlc_elab++subst_eval_ctx_elab ++ stlc_elab))
-       As subst_Estlc_wf.
-Proof.
-  assert (elab_lang (subst_eval_ctx ++ stlc)
-                    (subst_eval_ctx_elab ++ stlc_elab)).
-  destruct TODO (*TODO: extension lemma for elab*).
-  match goal with
-  | [|- elab_lang ?l ?el] =>
-  rewrite (as_nth_tail l);
-    rewrite (as_nth_tail el)
-  end.
-  repeat ((eapply elab_lang_cons_nth_tail_app
-           || eapply elab_lang_cons_nth_tail);
-              [compute; reflexivity
-              | compute; reflexivity
-              | apply use_compute_fresh; compute; reflexivity
-              | ..]).
-  
-  rewrite !nth_tail_length_app; [assumption|..].
-  cbn.
-  match goal with
-    [ |-context [length ?emp]] => unify emp (@nil (string*rule))
-  end.
-  reflexivity.
-  reflexivity.
-
-  all:(unshelve solve[repeat t];
-  cleanup_auto_elab).
-Qed.
+       SuchThat (Pre.elab_lang (eval_ctx_elab ++ stlc_elab ++ subst_elab) Estlc Estlc_elab)
+       As Estlc_wf.
+Proof. auto_elab. Qed.
+#[export] Hint Resolve Estlc_wf : elab_pfs.
+ 
